provide implementations of abstract_env

safechecker/theories/PCUICWfEnvImpl.v
@@ -45,20 +45,36 @@ destruct (wf_ext_gc_of_uctx HΣ) as [uctx Huctx].
 exists (make_graph uctx). unfold is_graph_of_uctx. now rewrite Huctx.
 Defined.
 
-Definition abstract_env_graph {abstract_env_ext_impl : Type} 
-  `{abstract_env_ext_prop abstract_env_impl} X `{abstract_env_ext_correct abstract_env_impl X} 
-  {Σ} (wfΣ : abstract_env_ext_rel X Σ)
-  := projT1 (graph_of_wf_ext (abstract_env_ext_wf wfΣ)).
+Require Import Morphisms.
 
-Definition abstract_env_graph_wf {cf:checker_flags} {abstract_env_ext_impl : Type} 
-`{abstract_env_ext_prop abstract_env_impl} X `{abstract_env_ext_correct abstract_env_impl X} 
- {Σ} (wfΣ : abstract_env_ext_rel X Σ) := projT2 (graph_of_wf_ext (abstract_env_ext_wf wfΣ)).
+Instance consistent_proper : Proper (CS.Equal ==> iff) consistent.
+Proof.
+  intros c c' eq. rewrite /consistent.
+  now setoid_rewrite eq.
+Qed.
+
+Lemma on_udecl_mono {cf:checker_flags} {Σ : global_env} {wfΣ : wf Σ} : on_udecl Σ Monomorphic_ctx.
+Proof.
+  repeat split; cbn.
+  - intros i; rewrite LevelSetFact.empty_iff //.
+  - intros i; rewrite ConstraintSetFact.empty_iff //.
+  - red. rewrite /univs_ext_constraints /=. 
+    rewrite CS_union_empty.
+    apply wfΣ.
+Qed.
+
+Record referenced_impl_ext {cf:checker_flags} := {
+      referenced_impl_env_ext :> global_env_ext;
+      referenced_impl_ext_wf :> ∥ wf_ext referenced_impl_env_ext ∥;
+      referenced_impl_ext_graph := projT1 (graph_of_wf_ext referenced_impl_ext_wf);
+      referenced_impl_ext_graph_wf := projT2 (graph_of_wf_ext referenced_impl_ext_wf)
+  }.
 
 Record referenced_impl {cf:checker_flags} := {
-      referenced_impl_env :> global_env_ext;
-      referenced_impl_wf :> ∥ wf_ext referenced_impl_env ∥;
-      referenced_impl_graph_ := projT1 (graph_of_wf_ext referenced_impl_wf);
-      referenced_impl_graph_wf_ := projT2 (graph_of_wf_ext referenced_impl_wf)
+      referenced_impl_env :> global_env;
+      referenced_impl_wf :> ∥ wf referenced_impl_env ∥;
+      referenced_impl_graph := projT1 (graph_of_wf referenced_impl_wf);
+      referenced_impl_graph_wf := projT2 (graph_of_wf referenced_impl_wf)
   }.
 
 Axiom guard_impl : FixCoFix -> global_env_ext -> context -> mfixpoint term -> bool.
@@ -85,61 +101,96 @@ Proof.
       + eapply wf_ext_consistent; eauto. 
 Defined. 
 
-Definition canonincal_abstract_env_ext_struct {cf:checker_flags} :
-  abstract_env_ext_struct referenced_impl :=
-  {| abstract_env_lookup := fun Σ => lookup_env (referenced_impl_env Σ) ;
-     abstract_env_conv_pb_relb := fun Σ conv_pb => conv_pb_relb (referenced_impl_graph_ Σ) conv_pb ;
+Global Instance canonincal_abstract_env_ext_struct {cf:checker_flags} :
+  abstract_env_ext_struct referenced_impl_ext :=
+  {| abstract_env_lookup := fun Σ => lookup_env (referenced_impl_env_ext Σ) ;
+     abstract_env_conv_pb_relb := fun Σ conv_pb => conv_pb_relb (referenced_impl_ext_graph Σ) conv_pb ;
      abstract_env_compare_global_instance := fun Σ =>
-      compare_global_instance (referenced_impl_env Σ)
-                              (check_eqb_universe (referenced_impl_graph_ Σ));
-     abstract_env_level_mem := fun Σ => level_mem (referenced_impl_env Σ);
+      compare_global_instance (referenced_impl_env_ext Σ)
+                              (check_eqb_universe (referenced_impl_ext_graph Σ));
+     abstract_env_level_mem := fun Σ => level_mem (referenced_impl_env_ext Σ);
      abstract_env_ext_wf_universeb := fun Σ u => wf_universeb Σ u;
-     abstract_env_check_constraints := fun Σ => check_constraints (referenced_impl_graph_ Σ);
+     abstract_env_check_constraints := fun Σ => check_constraints (referenced_impl_ext_graph Σ);
 
-     abstract_env_guard := fun Σ fix_cofix => guard_impl fix_cofix (referenced_impl_env Σ);
-     abstract_env_ext_rel := fun X Σ => Σ = referenced_impl_env X
+     abstract_env_guard := fun Σ fix_cofix => guard_impl fix_cofix (referenced_impl_env_ext Σ);
+     abstract_env_ext_rel := fun X Σ => Σ = referenced_impl_env_ext X
   |}.
+
+Definition init_env : global_env := {| universes := (LS.singleton Level.lzero , CS.empty); declarations := [] |}.
+
+Definition on_global_univ_init : on_global_univs init_env.
+Admitted.
+
+Program Global Instance canonincal_abstract_env_struct {cf:checker_flags} :
+  abstract_env_struct referenced_impl referenced_impl_ext :=
+ {|
+ abstract_env_empty := {|
+ referenced_impl_env := init_env ;
+ |} ;
+ abstract_env_init := fun cs H =>  {|
+ referenced_impl_env := {| universes := cs ; declarations := [] |};
+ |} ;
+ abstract_env_add_decl := fun X kn d H => 
+  {| referenced_impl_env := add_global_decl X.(referenced_impl_env) (kn,d);
+   |};
+ abstract_env_empty_ext X := {| referenced_impl_env_ext := (X , Monomorphic_ctx);
+ |} ;
+ abstract_env_univ X := X ;
+ abstract_env_global_declarations X := declarations X;
+ abstract_env_is_consistent uctx := wGraph.is_acyclic (make_graph uctx);
+ abstract_env_is_consistent_uctx X uctx := wGraph.is_acyclic (add_uctx uctx (referenced_impl_graph X)) ;
+ abstract_env_add_uctx X uctx udecl Hdecl Hglobal := {| referenced_impl_env_ext := (X.(referenced_impl_env) , udecl);
+ |} ;
+ abstract_env_rel := fun X Σ => Σ = referenced_impl_env X
+ |}.
+Next Obligation. sq; constructor; cbn. 
+- apply on_global_univ_init.
+- econstructor.
+Qed.
+Next Obligation. sq; constructor; eauto. econstructor. Qed.
+Next Obligation. pose proof (referenced_impl_wf X) as [[? ?]]. sq. split; cbn; eauto.
+  destruct H; econstructor; eauto. 
+Qed.
+Next Obligation. pose proof (referenced_impl_wf X) as [?]. sq. split; eauto.
+  apply on_udecl_mono.
+Qed.   
+Next Obligation.
+  pose proof (referenced_impl_wf X). now sq.
+Qed.  
 
 (* We pack up all the information required on the global environment and graph in a
 single record. *)
 
 Record wf_env {cf:checker_flags} := {
-  wf_env_env :> global_env;
+  wf_env_referenced :> referenced_impl;
   wf_env_map :> EnvMap.t global_decl;
-  wf_env_map_repr :> EnvMap.repr wf_env_env.(declarations) wf_env_map;
-  wf_env_wf :> ∥ wf wf_env_env ∥;
-  wf_env_graph :> universes_graph;
-  wf_env_graph_wf : is_graph_of_uctx wf_env_graph (global_uctx wf_env_env)
+  wf_env_map_repr :> EnvMap.repr (referenced_impl_env wf_env_referenced).(declarations) wf_env_map;
 }.
 
 Record wf_env_ext {cf:checker_flags} := {
-  wf_env_ext_env :> global_env_ext;
+  wf_env_ext_referenced :> referenced_impl_ext;
   wf_env_ext_map :> EnvMap.t global_decl;
-  wf_env_ext_map_repr :> EnvMap.repr wf_env_ext_env.(declarations) wf_env_ext_map;
-  wf_env_ext_wf :> ∥ wf_ext wf_env_ext_env ∥;
-  wf_env_ext_graph :> universes_graph;
-  wf_env_ext_graph_wf : is_graph_of_uctx wf_env_ext_graph (global_ext_uctx wf_env_ext_env)
+  wf_env_ext_map_repr :> EnvMap.repr (referenced_impl_env_ext wf_env_ext_referenced).(declarations) wf_env_ext_map;
 }.
 
-Definition fake_guard_impl : FixCoFix -> global_env_ext -> context -> mfixpoint term -> bool
+(*
+ Definition fake_guard_impl : FixCoFix -> global_env_ext -> context -> mfixpoint term -> bool
   := fun fix_cofix Σ Γ mfix => true.
 
-Axiom fake_guard_correct : forall fix_cofix Σ Γ mfix,
+  Axiom fake_guard_correct : forall fix_cofix Σ Γ mfix,
   guard fix_cofix Σ Γ mfix <-> fake_guard_impl fix_cofix Σ Γ mfix.
+*)
 
-Definition optimized_abstract_env_ext_struct {cf:checker_flags} :
+Global Instance optimized_abstract_env_ext_struct {cf:checker_flags} :
   abstract_env_ext_struct wf_env_ext :=
   {| abstract_env_lookup := fun Σ k => EnvMap.lookup k (wf_env_ext_map Σ);
-     abstract_env_conv_pb_relb := fun Σ conv_pb => conv_pb_relb (wf_env_ext_graph Σ) conv_pb ;
-     abstract_env_compare_global_instance := fun Σ =>
-      compare_global_instance (wf_env_ext_env Σ)
-                              (check_eqb_universe (wf_env_ext_graph Σ));
-     abstract_env_level_mem := fun Σ l => LevelSet.mem l (uGraph.wGraph.V (wf_env_ext_graph Σ));
-     abstract_env_ext_wf_universeb := fun Σ u => wf_universeb Σ u;
-     abstract_env_check_constraints := fun Σ => check_constraints (wf_env_ext_graph Σ);
-
-     abstract_env_guard := fun Σ fix_cofix => fake_guard_impl fix_cofix (wf_env_ext_env Σ);
-     abstract_env_ext_rel := fun X Σ => Σ = wf_env_ext_env X
+     abstract_env_conv_pb_relb X := abstract_env_conv_pb_relb X.(wf_env_ext_referenced);
+     abstract_env_compare_global_instance X := abstract_env_compare_global_instance X.(wf_env_ext_referenced);
+     abstract_env_level_mem X := abstract_env_level_mem X.(wf_env_ext_referenced);
+     abstract_env_ext_wf_universeb X := abstract_env_ext_wf_universeb X.(wf_env_ext_referenced);
+     abstract_env_check_constraints X := abstract_env_check_constraints X.(wf_env_ext_referenced);
+     abstract_env_guard X := abstract_env_guard X.(wf_env_ext_referenced);
+     abstract_env_ext_rel X := abstract_env_ext_rel X.(wf_env_ext_referenced);
   |}.
 
   Lemma wf_fresh_globals {cf : checker_flags} Σ : wf Σ -> EnvMap.fresh_globals Σ.(declarations).
@@ -153,24 +204,53 @@ Proof.
   reflexivity.
 Qed.
 
+Program Definition wf_env_empty {cf:checker_flags} : wf_env := 
+{|   
+  wf_env_referenced := abstract_env_empty;
+  wf_env_map := EnvMap.empty;
+  |}.
+
+Program Definition wf_env_init {cf:checker_flags} cs : 
+  on_global_univs cs -> wf_env := fun H =>
+  {|   
+  wf_env_referenced := abstract_env_init cs H;
+  wf_env_map := EnvMap.empty;
+  |}.
+
+Program Global Instance optimized_abstract_env_struct {cf:checker_flags} :
+  abstract_env_struct wf_env wf_env_ext :=
+ {|
+ abstract_env_empty := wf_env_empty;
+ abstract_env_init := wf_env_init;
+ abstract_env_add_decl X kn d H :=
+  {| wf_env_referenced := @abstract_env_add_decl _ _ referenced_impl_ext _ X.(wf_env_referenced) kn d H ;
+     wf_env_map := EnvMap.add kn d X.(wf_env_map) |};
+ abstract_env_empty_ext X := 
+  {| wf_env_ext_referenced := @abstract_env_empty_ext _ _ referenced_impl_ext _ X.(wf_env_referenced) ;
+     wf_env_ext_map := X.(wf_env_map) |};
+ abstract_env_global_declarations X := abstract_env_global_declarations X.(wf_env_referenced);
+ abstract_env_is_consistent univ := abstract_env_is_consistent univ;
+ abstract_env_is_consistent_uctx X uctx := abstract_env_is_consistent_uctx X.(wf_env_referenced) uctx;
+ abstract_env_add_uctx X uctx udecl Huctx Hdecl := 
+ {| wf_env_ext_referenced := @abstract_env_add_uctx _ _ referenced_impl_ext _ X.(wf_env_referenced) uctx udecl Huctx Hdecl ;
+    wf_env_ext_map := X.(wf_env_map) |};
+ abstract_env_rel X := abstract_env_rel X.(wf_env_referenced)
+ |}.
+Next Obligation.
+  pose proof (X.(wf_env_referenced).(referenced_impl_wf)) as [?].
+  sq. destruct H.  
+  apply EnvMap.repr_add; eauto; try eapply wf_fresh_globals; eauto. 
+  apply wf_env_map_repr.
+Defined. 
+Next Obligation. apply wf_env_map_repr. Defined.
+Next Obligation. apply wf_env_map_repr. Defined.
+
 Section WfEnv.
   Context {cf : checker_flags}.
 
-  Definition wf_env_sq_wf (Σ : wf_env) : ∥ wf Σ ∥.
+  Definition referenced_impl_sq_wf (Σ : referenced_impl_ext) : ∥ wf Σ ∥.
   Proof.
-    destruct (wf_env_wf Σ).
-    sq. apply X.
-  Qed.
-
-  Definition wf_env_ext_sq_wf (Σ : wf_env_ext) : ∥ wf Σ ∥.
-  Proof.
-    destruct (wf_env_ext_wf Σ).
-    sq. apply X.
-  Qed.
-
-  Definition referenced_impl_sq_wf (Σ : referenced_impl) : ∥ wf Σ ∥.
-  Proof.
-    destruct (referenced_impl_wf Σ).
+    destruct (referenced_impl_ext_wf Σ).
     sq. apply X.
   Qed.
 
@@ -179,8 +259,8 @@ Section WfEnv.
 
   Lemma lookup_lookup_env Σ kn : lookup Σ kn = lookup_env Σ kn.
   Proof.
-    rewrite /lookup. destruct Σ as [Σ map repr [wfext] G HG].
-    apply EnvMap.lookup_spec; auto. now eapply wf_fresh_globals.
+    rewrite /lookup. destruct Σ as [Σ map repr]. pose (referenced_impl_sq_wf Σ).
+    sq. apply EnvMap.lookup_spec; auto. now eapply wf_fresh_globals.
   Qed.
 
 End WfEnv.
@@ -190,21 +270,16 @@ Create HintDb wf_env discriminated.
 Global Hint Constants Opaque : wf_env.
 Global Hint Variables Opaque : wf_env.
 
-Global Hint Resolve wf_env_ext_wf : wf_env.
+Global Hint Resolve referenced_impl_ext_wf : wf_env.
+Global Hint Resolve referenced_impl_wf : wf_env.
 
-Ltac unsquash_wf_env :=
-  match goal with
-  | Σ : wf_env_ext |- _ => try destruct Σ.(wf_env_ext_wf) as [wfΣ]
-  end.
-
-Global Hint Resolve wf_env_ext_sq_wf : wf_env.
-Global Hint Resolve wf_env_ext_graph_wf : wf_env.
-
-Definition Σudecl {cf : checker_flags} (Σ : wf_env_ext) : ∥ on_udecl Σ.(wf_env_ext_env).1 Σ.(wf_env_ext_env).2 ∥ :=
-  map_squash (fun x => x.2) Σ.
-
-Definition Σudecl_ref {cf : checker_flags} (Σ : referenced_impl) : ∥ on_udecl Σ.(referenced_impl_env).1 Σ.(referenced_impl_env).2 ∥ :=
+Definition Σudecl_ref {cf : checker_flags} (Σ : referenced_impl_ext) : 
+  ∥ on_udecl Σ.(referenced_impl_env_ext).1 Σ.(referenced_impl_env_ext).2 ∥ :=
     map_squash (fun x => x.2) Σ.
+
+Definition Σudecl {cf : checker_flags} (Σ : wf_env_ext) : 
+  ∥ on_udecl Σ.(referenced_impl_env_ext).1 Σ.(referenced_impl_env_ext).2 ∥ :=
+  map_squash (fun x => x.2) Σ.
   
   Global Hint Resolve Σudecl : wf_env.
 
@@ -216,12 +291,11 @@ Ltac wf_env := auto with wf_env.
   convertible to [Σ]. *)
 
 Definition build_wf_env_ext {cf : checker_flags} (Σ : global_env_ext) (wfΣ : ∥ wf_ext Σ ∥) : wf_env_ext :=
-  {| wf_env_ext_env := Σ;
+  {| wf_env_ext_referenced := 
+      {| referenced_impl_env_ext := Σ; referenced_impl_ext_wf := wfΣ |} ;
      wf_env_ext_map := EnvMap.of_global_env Σ.(declarations);
      wf_env_ext_map_repr := EnvMap.repr_global_env Σ.(declarations);
-     wf_env_ext_wf := wfΣ;
-     wf_env_ext_graph := projT1 (graph_of_wf_ext wfΣ);
-     wf_env_ext_graph_wf := projT2 (graph_of_wf_ext wfΣ) |}.
+|}.
 
 Section GraphSpec.
   Context {cf:checker_flags} {Σ : global_env_ext} (HΣ : ∥ wf Σ ∥)
@@ -243,22 +317,17 @@ Section GraphSpec.
     sq; now eapply global_ext_uctx_consistent.
   Qed. 
 
-  Lemma check_constraints_complete ctrs (H : check_univs)
-  : valid_constraints (global_ext_constraints Σ) ctrs -> check_constraints G ctrs.
+  Lemma check_constraints_complete ctrs (H : check_univs) :
+  uctx_invariants ((global_ext_uctx Σ).1, ctrs) -> valid_constraints (global_ext_constraints Σ) ctrs -> check_constraints G ctrs.
   Proof.
     pose proof HΣ'.
-    intros HH.
+    intros Huctx HH.  
     refine (check_constraints_complete G (global_ext_uctx Σ) _ _ HG _ _ _ HH); eauto; sq.
     now eapply wf_ext_global_uctx_invariants.
     now eapply global_ext_uctx_consistent.
     pose proof (wf_ext_global_uctx_invariants Σ H0) as [H1 H2].
-    split; eauto. clear H1. 
-    unfold uctx_invariants in *; cbn in *.   
-    unfold valid_constraints in HH. rewrite H in HH.
-    unfold valid_constraints0 in HH. unfold ConstraintSet.For_all.
-    intro x; specialize (H2 x). intro; apply H2.
-    
-  Admitted.
+    split; eauto.
+  Defined.
 
   Lemma is_graph_of_uctx_levels (l : Level.t) :
     LevelSet.mem l (uGraph.wGraph.V G) <->
@@ -277,14 +346,16 @@ Section GraphSpec.
 End GraphSpec.
 
 
-Program Definition canonincal_abstract_env_prop {cf:checker_flags} :
+Program Global Instance canonincal_abstract_env_ext_prop {cf:checker_flags} :
   @abstract_env_ext_prop _ _ canonincal_abstract_env_ext_struct :=
-     {| abstract_env_ext_exists := fun Σ => sq (referenced_impl_env Σ ; eq_refl); |}.
-Next Obligation. apply check_conv_pb_relb_correct; eauto. apply referenced_impl_wf. apply referenced_impl_graph_wf_.  Defined.
+     {| abstract_env_ext_exists := fun Σ => sq (referenced_impl_env_ext Σ ; eq_refl); |}.
+Next Obligation. wf_env. Defined.
+Next Obligation. apply check_conv_pb_relb_correct; eauto; wf_env.   
+   apply (graph_of_wf_ext X).π2. Defined.
 Next Obligation. eapply reflect_iff. eapply reflect_R_global_instance; eauto.
   move => ? ? /wf_universe_reflect ? - /wf_universe_reflect ?.
-  apply iff_reflect;  apply check_conv_pb_relb_correct with (conv_pb := Conv); eauto.
-  apply referenced_impl_wf. apply referenced_impl_graph_wf_.
+  apply iff_reflect;  apply check_conv_pb_relb_correct with (conv_pb := Conv); eauto; wf_env. 
+  apply (graph_of_wf_ext X).π2.
   move => ? ? /wf_universe_reflect ? - /wf_universe_reflect ?.
   apply X0; eauto. 
   all: rewrite wf_universeb_instance_forall.
@@ -294,54 +365,77 @@ Defined.
 Next Obligation. split; intros. 
   - eapply check_constraints_complete; eauto.
     apply referenced_impl_sq_wf. apply Σudecl_ref.
-    apply referenced_impl_graph_wf_.
+    apply (graph_of_wf_ext X).π2.
+    now destruct X. 
   - eapply check_constraints_spec; eauto.    
   apply referenced_impl_sq_wf. apply Σudecl_ref.
-  apply referenced_impl_graph_wf_.
+  apply (graph_of_wf_ext X).π2.
   Defined. 
 Next Obligation. apply guard_correct. Defined.
 
-Program Definition canonincal_abstract_env_correct {cf:checker_flags}
-  (X : referenced_impl) :
-  @abstract_env_ext_correct _ cf canonincal_abstract_env_ext_struct X.
-Proof. econstructor. intros. cbn in H; subst. apply referenced_impl_wf. Defined.
-
-
-Program Definition optimized_abstract_env_prop {cf:checker_flags} :
+Program Global Instance optimized_abstract_env_extprop {cf:checker_flags} :
 @abstract_env_ext_prop _ _ optimized_abstract_env_ext_struct :=
-   {| abstract_env_ext_exists := fun Σ => sq (wf_env_ext_env Σ ; eq_refl); |}.
-Next Obligation. pose (wf_env_ext_wf X). sq. 
+   {| abstract_env_ext_exists := fun Σ => sq (referenced_impl_env_ext Σ ; eq_refl); |}.
+Next Obligation. wf_env. Defined.
+Next Obligation. pose (referenced_impl_ext_wf X). sq. 
   erewrite EnvMap.lookup_spec; try reflexivity. 
   1: apply wf_fresh_globals; eauto.
   1: apply wf_env_ext_map_repr. Qed.
-Next Obligation. apply check_conv_pb_relb_correct; eauto.
-  apply wf_env_ext_wf. apply wf_env_ext_graph_wf.
-Defined.
-Next Obligation. eapply reflect_iff. eapply reflect_R_global_instance; eauto.
-  move => ? ? /wf_universe_reflect ? - /wf_universe_reflect ?.
-  apply iff_reflect;  apply check_conv_pb_relb_correct with (conv_pb := Conv); eauto.
-  apply wf_env_ext_wf. apply wf_env_ext_graph_wf.
-  move => ? ? /wf_universe_reflect ? - /wf_universe_reflect ?.
-  apply X0; eauto. 
-  all: rewrite wf_universeb_instance_forall.
-  revert H; move => / wf_universe_instanceP ?; eauto. 
-  revert H0; move => / wf_universe_instanceP ?; eauto. 
-Defined. 
-Next Obligation. eapply eq_true_iff_eq.
-                 split; intros; eapply is_graph_of_uctx_levels; eauto;
-                 eapply wf_env_ext_graph_wf. Qed.
-Next Obligation. split; intros. 
-  - eapply check_constraints_complete; eauto.
-    apply wf_env_ext_sq_wf. apply Σudecl.
-    apply wf_env_ext_graph_wf.
-  - eapply check_constraints_spec; eauto.    
-    apply wf_env_ext_sq_wf. apply Σudecl.
-    apply wf_env_ext_graph_wf.
-Defined. 
-Next Obligation. apply fake_guard_correct. Defined.
+Next Obligation. now rewrite (abstract_env_compare_universe_correct X.(wf_env_ext_referenced)). Defined.
+Next Obligation. now rewrite (abstract_env_compare_global_instance_correct X.(wf_env_ext_referenced)); eauto. Defined.
+Next Obligation. now rewrite (abstract_env_check_constraints_correct X.(wf_env_ext_referenced)); eauto. Defined.
+Next Obligation. now rewrite (abstract_env_guard_correct X.(wf_env_ext_referenced)); eauto. Defined.
 
-Program Definition optimized_abstract_env_correct {cf:checker_flags} 
-  (X : wf_env_ext):
-  @abstract_env_ext_correct _ cf optimized_abstract_env_ext_struct X.
-Proof. econstructor. intros. cbn in H; subst. apply wf_env_ext_wf. Defined.
+Program Global Instance canonincal_abstract_env_prop {cf:checker_flags} :
+  @abstract_env_prop _ _ _ canonincal_abstract_env_ext_struct canonincal_abstract_env_struct.
+Next Obligation. now sq. Qed.
+Next Obligation. wf_env. Qed.
+Next Obligation. now split. Qed.
+Next Obligation. now split. Qed.
+Next Obligation. unshelve epose proof (is_consistent_spec udecl _) as Hconsistent; eauto.
+  unfold is_consistent in Hconsistent; now rewrite H0 in Hconsistent.
+  Qed.
+Next Obligation. 
+  rename H1 into Huctx. unfold referenced_impl_graph.
+  pose proof (referenced_impl_graph_wf X) as HG.
+  set (gph := (graph_of_wf X).π1) in *. clearbody gph. simpl in HG.  
+  unfold is_graph_of_uctx in HG. unfold gc_of_uctx in *.
+  case_eq (gc_of_constraints (global_uctx X).2).
+  2:{ intro XX. rewrite XX in HG. inversion HG. }
+  intros Σctrs HΣctrs.
+  rewrite HΣctrs in HG. simpl in HG.
+  case_eq (gc_of_constraints (constraints_of_udecl udecl));
+    [|intro XX; rewrite XX in Huctx; discriminate Huctx].
+  intros ctrs Hctrs. rewrite Hctrs in Huctx. simpl in *.
+  rewrite - (is_consistent_spec (global_ext_uctx (X, udecl))).
+  pose proof (gc_of_constraints_union (constraints_of_udecl udecl) (global_constraints X)).
+  rewrite {}HΣctrs {}Hctrs in H. simpl in H.
+  unfold is_consistent, global_ext_uctx, gc_of_uctx, global_ext_constraints. simpl. 
+  destruct (gc_of_constraints (ConstraintSet.union (constraints_of_udecl udecl)
+  (global_constraints X))).
+  - simpl in H. inversion Huctx; subst; clear Huctx. 
+  clear -H H0 cf HG.   
+  rewrite -HG add_uctx_make_graph. 
+  unfold global_ext_levels, global_levels in *. simpl.
+  assert (make_graph
+  (LevelSet.union (levels_of_udecl udecl)
+     (LevelSet.union (ContextSet.levels X) (LevelSet.singleton Level.lzero)),
+  t1) =_g make_graph
+  (LevelSet.union (levels_of_udecl udecl)
+     (LevelSet.union (ContextSet.levels X) (LevelSet.singleton Level.lzero)),
+     GoodConstraintSet.union t0 Σctrs)).
+  { apply make_graph_proper. now split; eauto. }     
+  now erewrite is_acyclic_proper.
+  - inversion H. 
+  Qed.   
 
+Program Global Instance optimized_abstract_env_prop {cf:checker_flags} :
+  @abstract_env_prop _ _ _ optimized_abstract_env_ext_struct optimized_abstract_env_struct.
+Next Obligation. now sq. Qed.
+Next Obligation. wf_env. Qed.
+Next Obligation. now split. Qed.
+Next Obligation. now split. Qed.
+Next Obligation. now erewrite (@abstract_env_is_consistent_correct _ _ _ _ _ canonincal_abstract_env_prop); eauto. Qed.
+Next Obligation. now erewrite (abstract_env_is_consistent_uctx_correct X.(wf_env_referenced)); eauto. Qed.
+  
+  
